Update test file (TODO: suppress test printing)

src/Pyrosome/Tools/EGraph/Test.v
@@ -75,13 +75,13 @@ Definition ex1_set :=
 Notation process_const_rules := (process_const_rules _ _ string_succ "v0" _ _ _ _ unit).
 Notation increment_epoch := (increment_epoch _ string_succ _ _ _ _).
 Notation run1iter :=
-  (run1iter _ _ string_succ "v0" _ _ _ _ _ _ _ unit (@PositiveInstantiation.compat_intersect)).
+  (run1iter _ _ string_succ "v0" _ _ _ _ _ _ _ _ (@PosListMap.compat_intersect)).
 
 Definition ex0 :=
   Eval vm_compute in
     (snd (Mseq (process_const_rules ex1_set)
             (rebuild 1000)
-            (empty_egraph default _))).
+            (empty_egraph _ _))).
 
 Ltac test H :=
   let H' := fresh in
@@ -114,8 +114,8 @@ Compute (map.tuples ex1.(parents _ _ _ _ _)).
 Definition ex1_graph :=
   Eval vm_compute in
     (snd (saturate_until string_succ "v0"
-       (@PositiveInstantiation.compat_intersect) ex1_set (Mret false) 5
-       (empty_egraph default _))).
+       (@PosListMap.compat_intersect) ex1_set (Mret false) 5
+       (empty_egraph _ _))).
 
 (*
 Compute (map (fun '(x,y) => (x, map.tuples y)) (map.tuples ex1_graph.(db _ _ _ _ _))).
@@ -150,8 +150,8 @@ Definition ex2_set :=
 Definition ex2_graph :=
   Eval native_compute in
     (snd (saturate_until string_succ "v0"
-       (@PositiveInstantiation.compat_intersect) ex2_set (Mret false) 0
-       (empty_egraph default _))).
+       (@PosListMap.compat_intersect) ex2_set (Mret false) 0
+       (empty_egraph _ _))).
 
 (*
 Compute (map (fun '(x,y) => (x, map.tuples y)) (map.tuples ex2_graph.(db _ _ _ _ _))).
@@ -176,7 +176,7 @@ Arguments run_query' {idx}%type_scope {Eqb_idx} {symbol}%type_scope
   {symbol_map}%function_scope {symbol_map_plus} {idx_map}%function_scope {idx_map_plus}
   {idx_trie}%function_scope  {analysis_result}%type_scope rs n%nat_scope _.
 
-Notation run_query := (run_query (@PositiveInstantiation.compat_intersect)).
+Notation run_query := (run_query (@PosListMap.compat_intersect)).
 Notation run_query' := (run_query').
 Notation build_tries := (build_tries _ _ _ _ _ _ _ _).
 
@@ -248,19 +248,19 @@ Definition monoid_ex1_rule_set :=
 Definition monoid_ex1_base :=
   Eval vm_compute in
     (snd (saturate_until string_succ "v0"
-       (@PositiveInstantiation.compat_intersect) monoid_ex1_rule_set (Mret false) 0
-       (empty_egraph default _))).
+       (@PosListMap.compat_intersect) monoid_ex1_rule_set (Mret false) 0
+       (empty_egraph _ _))).
       
 Definition monoid_ex1_graph :=
   Eval vm_compute in
     (snd (saturate_until string_succ "v0"
-       (@PositiveInstantiation.compat_intersect) monoid_rule_set_full (Mret false) 2
+       (@PosListMap.compat_intersect) monoid_rule_set_full (Mret false) 2
        monoid_ex1_base)).
 (*TODO: seems to work!
 Definition monoid_ex1_graph' :=
   Eval vm_compute in
     (snd (saturate_until string_succ "v0"
-       (@PositiveInstantiation.compat_intersect) monoid_rule_set (Mret false) 2
+       (@PosListMap.compat_intersect) monoid_rule_set (Mret false) 2
        monoid_ex1_graph)).
 *)
 (*
@@ -304,13 +304,13 @@ Definition ne_firstn {A} n (l : ne_list A) : ne_list A :=
   (fst l, firstn n (snd l)).
 
 (*
-Compute (intersection_keys string _ (@PositiveInstantiation.compat_intersect)
+Compute (intersection_keys string _ (@PosListMap.compat_intersect)
            (ne_firstn 0 tries)).
-Compute (intersection_keys string _ (@PositiveInstantiation.compat_intersect)
+Compute (intersection_keys string _ (@PosListMap.compat_intersect)
            (ne_firstn 1 tries)).
 
-Compute (map.tuples (PositiveInstantiation.proj_node_map
-           (PositiveInstantiation.compat_intersect (fun _ _ : unit => tt)
+Compute (map.tuples (PosListMap.proj_node_map
+           (PosListMap.compat_intersect (fun _ _ : unit => tt)
            (ne_firstn 0 tries)) : string_trie_map _)).
 *)
 (*
@@ -338,7 +338,7 @@ Compute (map.tuples ex2_graph.(parents _ _ _ _ _)).
 
 
 (*
-Import PositiveInstantiation.
+Import PosListMap.
 Local Existing Instance pos_trie_map.
 (* expect ["foo"; "foo"]*)
 Goal
@@ -420,9 +420,9 @@ Definition logic : lang string :=
 
 
 Eval vm_compute in
-    (map (uncurry (rule_to_log_rule (@StringInstantiation.string_trie_map)
-                     (@StringInstantiation.string_list_trie_map)
-                     StringInstantiation.string_succ "sort_of"
+    (map (uncurry (rule_to_log_rule (string_ptree_map_plus)
+                     (@StringListMap.string_list_trie_map)
+                     StringListMap.string_succ "sort_of"
                      logic (analysis_result:=unit))) logic).
 
 (*TODO: foo, bar rules not simplified.
@@ -456,8 +456,8 @@ Definition logic_rule_set :=
 Definition logic_ex1_base :=
   Eval vm_compute in
     (snd (saturate_until string_succ "v0"
-       (@PositiveInstantiation.compat_intersect) logic_rule_set_full (Mret false) 1
-       (empty_egraph default _))).
+       (@PosListMap.compat_intersect) logic_rule_set_full (Mret false) 1
+       (empty_egraph _ _))).
 Compute (map (fun '(x,y) => (x, map.tuples y)) (map.tuples logic_ex1_base.(db))).
 Compute (filter (fun p => negb (eqb (fst p) (snd p)))
            (map.tuples monoid_ex1_base.(equiv).(UnionFind.parent _ _ _))).
@@ -465,9 +465,352 @@ Compute (filter (fun p => negb (eqb (fst p) (snd p)))
 Definition logic_ex1_graph :=
   Eval native_compute in
     (snd (saturate_until string_succ "v0"
-       (@PositiveInstantiation.compat_intersect) logic_rule_set (Mret false) 5
+       (@PosListMap.compat_intersect) logic_rule_set (Mret false) 5
        logic_ex1_base)).
 (*TODO: why no unifications?*)
 Compute (filter (fun p => negb (eqb (fst p) (snd p)))
            (map.tuples monoid_ex1_base.(equiv).(UnionFind.parent _ _ _))).
 
+Require Import BinNums Defs.
+Import PosListMap.
+Instance my_analysis {V} : analysis V V _ := weighted_depth_analysis (fun _ => Some xH).
+Require Tools.UnElab.
+
+
+  Arguments Defs.run1iter {idx}%type_scope {Eqb_idx} idx_succ%function_scope 
+  idx_zero {symbol}%type_scope {Eqb_symbol} {symbol_map}%function_scope symbol_map_plus
+  {idx_map}%function_scope idx_map_plus {idx_trie}%function_scope {analysis_result}%type_scope 
+  {H} spaced_list_intersect%function_scope rs rebuild_fuel%nat_scope _.
+
+Ltac egraph n :=
+      lazymatch goal with
+        |- eq_term ?l ?c ?t ?e1 ?e2 =>
+          let l' := constr:(ctx_to_rules c ++ l) in
+          let rs := constr:(StringInstantiation.build_rule_set
+                              (PositiveInstantiation.filter_eqn_rules l') l') in
+          
+        let result := (eval vm_compute in
+                        (StringInstantiation.egraph_equal (X:= option positive) (*V:=string*) l' rs n c e1 e2 t)) in
+          let result' := eval vm_compute in
+          (Defs.run1iter string_succ "v0" string_ptree_map_plus string_ptree_map_plus
+             (@compat_intersect) rs 0 (snd result)
+          ) in
+        lazymatch result with
+        | (?b, ?g (*, ?r *)) =>
+            (*
+            (*TODO: how to extract and then rename?*)
+            let lp_and_r' := constr:((rename_lang (ctx_to_rules c ++ l) r)) in
+            let e1p := constr:(rename_term (var_to_con e1) (snd lp_and_r')) in
+             *)
+            (*
+            let p :=
+              (eval native_compute in (
+                  let (x1,g0) := add_open_term Pos.succ sort_of (fst lp_and_r')
+                                   [] (fst e1p) g in
+                  (x1,extract_weighted subst_weight 1000 g0 x1)
+              ))
+            in
+            match p with
+            | (?x1,?e1') =>*)
+       (* let assign := eval vm_compute in (fst (run_query (@PosListMap.compat_intersect) rw1 7 g)) in*)
+            pose (GoalDisplay.lie_to_user (real:=g) tt) as graph;
+            let rs' := eval vm_compute in
+            (named_map map.tuples (map.tuples rs.(query_clauses _ _ _ _)),
+              rs.(compiled_rules _ _ _ _)
+            ) in
+            pose (GoalDisplay.lie_to_user (real:=rs) tt) as rws;
+           
+                 (*pose (lie_to_user (real:=rw1) tt) as rules;*)
+                 idtac b (*"! Also," e1 "became" e1' "with id" x1
+        end*)
+         
+        | _ => fail "ill-formed!"
+        end
+      end.
+
+Definition print_egraph {X} (g : instance string string string_trie_map string_trie_map string_list_trie_map X) :=
+  (named_map (named_map (entry_value _ X)) (named_map map.tuples (map.tuples g.(db))),
+    map.tuples g.(equiv).(parent _ _ _)).
+
+    (*TODO: debug rules?*)
+(* TODO: think about variable order for query performance
+
+   TODO: extract now takes all of my ram.
+ *)
+(*
+Goal eq_term logic {{c  "a": #"S", "b" : #"S" }}
+  {{s #"S" }}
+  {{e #"/\" (#"/\" (#"-" #"F") "b") "a" }}
+  {{e #"/\" "b" (#"/\" "a" "a") }}.
+ *)
+
+Ltac print_rules :=
+ 
+lazymatch goal with
+  |- eq_term ?l ?c ?t ?e1 ?e2 =>
+    let l' := constr:(ctx_to_rules c ++ l) in
+    let r :=  eval vm_compute in
+    (map (uncurry (rule_to_log_rule (string_ptree_map_plus)
+                     (@StringListMap.string_list_trie_map)
+                     StringListMap.string_succ "@sort_of"
+                     l' (analysis_result:=unit))) (PositiveInstantiation.filter_eqn_rules l')) in
+        idtac r
+end.
+
+
+Goal eq_term logic {{c  "a": #"S", "b" : #"S" }}
+  {{s #"S" }}
+  {{e #"/\" (#"/\" (#"-" #"F") "b") "a" }}
+  {{e #"/\" "b" (#"/\" "a" "a") }}.
+
+
+  egraph 10.
+  Compute (map.get graph.(analyses _ _ _ _ _ _) "#9").
+  (*TODO: 9 can be xO xH here, why is it xI xH?*)
+  (* issue: 9 different after 2nd iter, not updated in db,
+     but 5 does get updated correctly
+   *)
+  
+  Compute (print_egraph graph).
+  Compute (map.tuples graph.(parents)).
+  Compute  (named_map map.tuples (map.tuples (graph.(db)))).
+  Compute (analyze _ _ _ (analysis:= my_analysis)
+             (Build_atom "/\" ["#10"; "#5"] "#9") [Some xH; Some xH]).
+
+  (*(*TODO: extraction is broken*)
+  TODO: is the analysis not updated in order to not update the epoch?.
+  Need an analysis rebuilding.
+  Probably best to keep separate since it's strictly simpler tha ngeneral rebuilding.
+  idea: after an analysis update, make sure to update parents.
+
+  Is this the problem?.
+  wouldn't this mean that the top-level analyses aren't updated?.
+  but the problem is that they are out of sync*)
+  lazymatch goal with
+  |- eq_term ?l ?c ?t ?e1 ?e2 =>
+    let l' := constr:(ctx_to_rules c ++ l) in
+    
+  let e' := eval vm_compute in
+  (let (x1,g0) := add_open_term StringListMap.string_succ
+                    StringListMap.sort_of l' true
+                    [] (var_to_con e1) graph in
+   let (x2,g1) := add_open_term StringListMap.string_succ
+                    StringListMap.sort_of l' true
+                    [] (var_to_con e2) graph in
+  ((unwrap_with_default (extract_weighted g0 1000 x1)), x1,
+             (unwrap_with_default (extract_weighted g1 1000 x2)), x2
+  )) in
+    idtac e'
+  end.
+  (*
+  Compute (print_egraph graph).
+  Compute (map.tuples graph.(parents)).
+*)
+  (*TODO: did something get unioned the wrong way? 7 still has its parents, as does 10.
+  the 7,9 union should have merged them*)
+  Compute (print_egraph graph).
+  Compute (map.tuples graph.(parents)).
+  Compute graph.(worklist).
+  Compute (map.tuples graph.(parents)).
+
+  Compute (print_egraph (snd (rebuild 100 graph))).
+  (*
+  TODO: rebuild doesn't do anything when it should; 7 non-canonical.
+  Note: wrong, but might be harmless?
+  TODO: not fully rebuilt!!!
+          TODO: sort of 7 is 10. what is 10?.
+  Note: above will be resolved on full rebuilding
+              *)
+print_rules.
+(*TODO: still have bug on T rule*)
+  pose (
+   (!! "#1" = "#2", "@sort_of" "#2" -> "" :- "/\" "#1" "#" -> "#2", "S" -> "", 
+     "F" -> "#1", "@sort_of" "#" -> "")%log) as seq.
+  
+
+  (* TODO: issue not with filter! why is there no #2 in the conclusion eqs?
+     where did #2 come from? did something not do a proper subst?
+   *)
+  Compute (QueryOpt.optimize_sequent string string_Eqb
+      StringListMap.string_succ string_default string string_Eqb
+      StringListMap.string_trie_map StringListMap.string_trie_map
+      string_ptree_map_plus
+      StringListMap.string_list_trie_map seq).
+  Compute (QueryOpt.opt_verbose string string_Eqb
+      StringListMap.string_succ string_default string string_Eqb
+      StringListMap.string_trie_map StringListMap.string_trie_map
+      string_ptree_map_plus
+      StringListMap.string_list_trie_map seq).
+  
+  
+  Compute (QueryOpt.opt_live_eqn string string_Eqb
+      StringListMap.string_succ string_default string string_Eqb
+      StringListMap.string_trie_map StringListMap.string_trie_map
+      string_ptree_map_plus
+      StringListMap.string_list_trie_map seq "#1" "#0").
+
+  Compute (QueryOpt.opt_conclusion_atoms string string_Eqb
+      StringListMap.string_succ string_default string string_Eqb
+      StringListMap.string_trie_map StringListMap.string_trie_map
+      string_ptree_map_plus
+      StringListMap.string_list_trie_map seq).
+  (*
+  [{| atom_fn := "@sort_of"; atom_args := ["#2"]; atom_ret := "" |};
+        {| atom_fn := "@sort_of"; atom_args := ["#"]; atom_ret := "" |};
+        {| atom_fn := "F"; atom_args := []; atom_ret := "#0" |};
+        {| atom_fn := "S"; atom_args := []; atom_ret := "" |};
+        {| atom_fn := "/\"; atom_args := ["#"; "#0"]; atom_ret := "#2" |}] *)
+  assert (QueryOpt.opt_assumption_atoms string string_Eqb
+      StringListMap.string_succ string_default string string_Eqb
+      StringListMap.string_trie_map StringListMap.string_trie_map
+      StringListMap.string_list_trie_map seq = []).
+
+  {
+    unfold opt_assumption_atoms.
+Definition focus {A} (a:A) : Prop := False.
+Opaque focus.
+(*
+  
+  TODO: error! reflexivity for #2 not included in assumptions!.
+  How is that possible w/ atom /\ 1 # -> 2?
+     = [{| atom_fn := "@sort_of"; atom_args := ["#"]; atom_ret := "" |};
+        {| atom_fn := "F"; atom_args := []; atom_ret := "#1" |};
+        {| atom_fn := "S"; atom_args := []; atom_ret := "" |};
+        {| atom_fn := "/\"; atom_args := ["#"; "#1"]; atom_ret := "#2" |}]
+
+    = [{| atom_fn := "@sort_of"; atom_args := ["#"]; atom_ret := "" |};
+        {| atom_fn := "F"; atom_args := []; atom_ret := "#1" |};
+        {| atom_fn := "S"; atom_args := []; atom_ret := "" |};
+        {| atom_fn := "/\"; atom_args := ["#"; "#1"]; atom_ret := "#2" |};
+        {| atom_fn := "@sort_of"; atom_args := ["#2"]; atom_ret := "" |};
+        {| atom_fn := "@sort_of"; atom_args := ["#"]; atom_ret := "" |};
+        {| atom_fn := "F"; atom_args := []; atom_ret := "#0" |};
+        {| atom_fn := "S"; atom_args := []; atom_ret := "" |};
+        {| atom_fn := "/\"; atom_args := ["#"; "#0"]; atom_ret := "#2" |}]
+    : list (atom string string)
+
+               = !! "#1" = "#0", "@sort_of" "#2" -> "" :- "/\" "#1" "#" -> "#2", 
+          "S" -> "", "F" -> "#1", "@sort_of" "#" -> ""
+  
+  Compute (QueryOpt.opt_known_atoms string string_Eqb
+      StringListMap.string_succ string_default string string_Eqb
+      StringListMap.string_trie_map StringListMap.string_trie_map
+      string_ptree_map_plus
+      StringListMap.string_list_trie_map seq).
+  TODO: issue w/ /\ false rule:
+      wrong unification. (1,0) should be (1,2).
+   Issue in erule compilation, specifically optimization
+  {|
+    query_vars := [""; "#2"; "#"; "#1"];
+    query_clause_ptrs :=
+      ({| query_ptr_symbol := "@sort_of"; query_ptr_ptr := ""; query_ptr_args := [""; "#"] |},
+       [{| query_ptr_symbol := "F"; query_ptr_ptr := ""; query_ptr_args := ["#1"] |};
+        {| query_ptr_symbol := "S"; query_ptr_ptr := ""; query_ptr_args := [""] |};
+        {| query_ptr_symbol := "/\"; query_ptr_ptr := "#"; query_ptr_args := ["#2"; "#"; "#1"] |}]);
+    write_vars := ["#0"];
+    write_clauses := [{| atom_fn := "@sort_of"; atom_args := ["#2"]; atom_ret := "" |}];
+    write_unifications := [("#1", "#0")]
+  |};
+   !! "#1" = "#2", "@sort_of" "#2" -> "" :- "/\" "#1" "#" -> "#2", "S" -> "", 
+    "F" -> "#1", "@sort_of" "#" -> "";
+  
+Compute (named_map (named_map (entry_value _ _))
+           (named_map map.tuples (map.tuples (graph.(db))))).
+(*TODO: still broken
+  ([("@sort_of", [("", ([1], 0))]); ("T", [("", ([], 0))]); ("F", [("", ([], 0))]);
+  ("-", [("", ([1], 0))]); ("S", [("", ([], 0))]); ("/\", [("#", ([1; 2], 0)); ("", ([1; 1], 0))])],*)
+
+
+lazymatch goal with
+  |- eq_term ?l ?c ?t ?e1 ?e2 =>
+    let l' := constr:(ctx_to_rules c ++ l) in
+    let r :=  eval vm_compute in
+    (map (uncurry (rule_to_log_rule (string_ptree_map_plus)
+                     (@StringListMap.string_list_trie_map)
+                     StringListMap.string_succ "@sort_of"
+                     l' (analysis_result:=unit))) (filter_eqn_rules l')) in
+        idtac r
+end.
+  
+([("@sort_of", [("", ([1], 0))]); ("T", [("", ([], 0))]); ("F", [("", ([], 0))]);
+  ("-", [("", ([1], 0))]); ("S", [("", ([], 0))]); ("/\", [("#", ([1; 2], 0)); ("", ([1; 1], 0))])],
+
+                                  
+                                  {|
+    query_vars := [""; "#2"; "#"; "#1"];
+    query_clause_ptrs :=
+      ({| query_ptr_symbol := "@sort_of"; query_ptr_ptr := ""; query_ptr_args := [""; "#"] |},
+       [{| query_ptr_symbol := "T"; query_ptr_ptr := ""; query_ptr_args := ["#1"] |};
+        {| query_ptr_symbol := "S"; query_ptr_ptr := ""; query_ptr_args := [""] |};
+        {| query_ptr_symbol := "/\"; query_ptr_ptr := "#"; query_ptr_args := ["#2"; "#"; "#1"] |}]);
+    write_vars := [];
+    write_clauses := [];
+    write_unifications := [("#1", ""); ("#", "#2")]
+                                  |};
+#1 = "", # = #2
+ :-
+ sort_of # -> "".
+ T -> #1.
+ S -> "".
+ /\ #1 # -> #2.
+                
+*)
+
+ 
+Compute (*(named_map (named_map (entry_value _ _))*)
+           (named_map map.tuples (map.tuples (graph.(db)))).
+(*TODO: fires when T in the LHS of /\.
+  Could this be a bug w/ dead var eqns on the write side?
+ *)
+
+(*
+lazymatch goal with
+  |- eq_term ?l ?c ?t ?e1 ?e2 =>
+    let l' := constr:(ctx_to_rules c ++ l) in
+    let r :=  eval vm_compute in
+    (map (uncurry (rule_to_log_rule (@StringListMap.string_trie_map)
+                     (@StringListMap.string_list_trie_map)
+                     StringListMap.string_succ "@sort_of"
+                     l' (analysis_result:=unit))) (filter_eqn_rules l')) in
+        idtac r
+end.
+lazymatch goal with
+  |- eq_term ?l ?c ?t ?e1 ?e2 =>
+    let l' := constr:(ctx_to_rules c ++ l) in
+    
+  let e' := eval vm_compute in
+  (let (x0,g0) := add_open_term StringListMap.string_succ
+                    StringListMap.sort_of l' true
+                    [] (var_to_con e1) graph in
+  let (x1,g1) := add_open_term StringListMap.string_succ
+                    StringListMap.sort_of l' true
+                    [] (var_to_con e1) graph in
+   (unwrap_with_default (extract_weighted g0 1000 x0),
+     unwrap_with_default (extract_weighted g1 1000 x1))) in
+    idtac e'
+end.
+*)
+
+(*
+ !! "#0" = "", "#1" = "#2", "#3" = "", "@sort_of" "#2" -> "" :- 
+    "/\" "#1" "#" -> "#2", "S" -> "", "F" -> "#1", "@sort_of" "#" -> "";
+ Check code path  for 0 = ""
+ !! "#0" = "", "#" = "#2" :- "/\" "#1" "#" -> "#2", "S" -> "", 
+    "T" -> "#1", "@sort_of" "#" -> "";
+ *)
+Compute (*(named_map (named_map (entry_value _ _))*)
+           (named_map map.tuples (map.tuples (graph.(db)))).
+                     
+Compute (map.tuples graph.(equiv).(parent _ _ _)).
+
+(*TODO: why false?
+  
+ *)
+Compute (fst (egraph_sort_of StringListMap.string_succ "@sort_of" "" "#5" graph)).
+
+(*TODO: issue: unified T and S! why?*)
+Compute (eq_proven StringListMap.string_succ "@sort_of" "" ""
+           "#5" graph).
+
+
+Abort.
